\documentclass[twoside,11pt]{article}
\usepackage{amsmath}
\usepackage{subcaption}
\usepackage[english]{babel}	
\usepackage{paralist}	
\usepackage[lowtilde]{url}
\usepackage{fixltx2e}
\usepackage{listings}
\usepackage{color}
\usepackage{hyperref}


\renewcommand{\thesubfigure}{\roman{subfigure}}
\definecolor{codegreen}{rgb}{0,0.6,0}
\definecolor{codegray}{rgb}{0.5,0.5,0.5}
\definecolor{codepurple}{rgb}{0.58,0,0.82}
\definecolor{backcolour}{rgb}{0.95,0.95,0.92}


\begin{document}
	
\title{Week 1}
\date{\vspace{-5ex}}
\maketitle

\section{Convexity}

\subsection{Exercise 1}

We will prove Jensen's inequality using induction.
For $m=2$ it holds from the definition of \emph{convex function}:
\begin{equation}
f(\lambda x_1 + (1 - \lambda) x_2) \leq \lambda f(x_1) + (1 - \lambda) f(x_2)
\end{equation}
Now, if for m=k is true we will prove that for m=k+1 is also true:
\begin{align}
	f\left(\sum_{i=1}^{k+1} \lambda_{i} x_{i}\right) & = f\left(\sum_{i=1}^{k} \lambda_{i} x_{i} + \lambda_{k+1}x_{k+1}\right) \\
	& = f\left(\left(\sum_{j=1}^{k} \lambda_j \right) \left(\sum_{i=1}^{k} \frac{\lambda_{i}}{\left(\sum_{j=1}^{k} \lambda_j \right)} x_{i} \right) + \lambda_{k+1}x_{k+1}\right) \\
	& \leq \left(\sum_{j=1}^{k} \lambda_j \right) f\left(\sum_{i=1}^{k} \frac{\lambda_{i}}{\left(\sum_{j=1}^{k} \lambda_j \right)} x_{i} \right) + \lambda_{k+1}f(x_{k+1}) \\ \label{use_cf_def_1}
	& \leq \sum_{i=1}^{k} \lambda_{i} f(x_{i}) + \lambda_{k+1}f(x_{k+1}) \\ \label{use_induction_1}
	& = \sum_{i=1}^{k+1} \lambda_{i} f(x_{i})
\end{align}
where in \eqref{use_cf_def_1}, we have used the fact that f is a convex function and in \eqref{use_induction_1}, that Jensen's inequality holds for m=k.

\subsection{Exercise 2}


	
\end{document}